bench_horn_ice/nonlin_minus_1.bpl
@@ -1,7 +1,7 @@
 // SMACK-PRELUDE-BEGIN
 procedure boogie_si_record_int(i: int);
 
-function {:existential true} b0(a:int, b:int, c:int, d:int, e:int): bool;
+function {:existential true} b0(a:int, b:int, n:int): bool;
 
 // Integer arithmetic
 function $add(p1:int, p2:int) returns (int) {p1 + p2}
@@ -155,32 +155,25 @@ procedure main()
 {
   var $a: int;
   var $b: int;
-  var $c1: int;
-  var $c2: int;
-  var $d1: int;
-  var $d2: int;
-  var $e1: int;
-  var $e2: int;
+  var $n: int;
+  var $n2: int;
+  var $a2: int;
 $bb0:
   assume $a > 0;
   assume $b > 0;
-  $c1 := 0;
-  $d1 := 0;
-  $e1 := 0;
+  $n := $mul($a, $b);
   goto $bb1;
 $bb1:
-  assert b0($a, $b, $c1, $d1, $e2);
+  assert b0($a, $b, $n);
   goto $bb2, $bb3;
 $bb2:
-  $c2 := $add($c1, 1);
-  $d2 := $add($d1, $a);
-  $e2 := $add($e1, $b);
-  $c1 := $c2;
-  $d1 := $d2;
-  $e1 := $e2;
+  $a2 := $sub($a, 1);
+  $n2 := $sub($n, $b);
+  $a := $a2;
+  $n := $n2;
   goto $bb1;
 $bb3:
-  assert ($mul($b, $c1) >= $mul($a, $c1));
+  assert ($n != 0) || ($a == 0);
   return;
 }
 
